libcrux-ml-kem/proofs/fstar/extraction/Libcrux_ml_kem.Simd.Simd128.fsti
@@ -1,0 +1,246 @@
+module Libcrux_ml_kem.Simd.Simd128
+#set-options "--fuel 0 --ifuel 1 --z3rlimit 15"
+open Core
+open FStar.Mul
+
+let v_BARRETT_MULTIPLIER: i32 = 20159l
+
+let v_INVERSE_OF_MODULUS_MOD_MONTGOMERY_R: i32 = 62209l
+
+val mask_n_least_significant_bits (coefficient_bits: i32)
+    : Prims.Pure i32 Prims.l_True (fun _ -> Prims.l_True)
+
+val montgomery_reduce_i32x2_t (v: Core.Core_arch.Arm_shared.Neon.t_int32x2_t)
+    : Prims.Pure Core.Core_arch.Arm_shared.Neon.t_int32x2_t Prims.l_True (fun _ -> Prims.l_True)
+
+val montgomery_reduce_i32x4_t (v: Core.Core_arch.Arm_shared.Neon.t_int32x4_t)
+    : Prims.Pure Core.Core_arch.Arm_shared.Neon.t_int32x4_t Prims.l_True (fun _ -> Prims.l_True)
+
+type t_SIMD128Vector = {
+  f_low:Core.Core_arch.Arm_shared.Neon.t_int32x4_t;
+  f_high:Core.Core_arch.Arm_shared.Neon.t_int32x4_t
+}
+
+val v_ZERO: Prims.unit -> Prims.Pure t_SIMD128Vector Prims.l_True (fun _ -> Prims.l_True)
+
+val add_constant (v: t_SIMD128Vector) (c: i32)
+    : Prims.Pure t_SIMD128Vector Prims.l_True (fun _ -> Prims.l_True)
+
+val add_vec (lhs rhs: t_SIMD128Vector)
+    : Prims.Pure t_SIMD128Vector Prims.l_True (fun _ -> Prims.l_True)
+
+val barrett_reduce (v: t_SIMD128Vector)
+    : Prims.Pure t_SIMD128Vector Prims.l_True (fun _ -> Prims.l_True)
+
+val bitwise_and_with_constant (v: t_SIMD128Vector) (c: i32)
+    : Prims.Pure t_SIMD128Vector Prims.l_True (fun _ -> Prims.l_True)
+
+val compress (v_COEFFICIENT_BITS: i32) (v: t_SIMD128Vector)
+    : Prims.Pure t_SIMD128Vector Prims.l_True (fun _ -> Prims.l_True)
+
+val compress_1_ (v: t_SIMD128Vector)
+    : Prims.Pure t_SIMD128Vector Prims.l_True (fun _ -> Prims.l_True)
+
+val cond_subtract_3329_ (v: t_SIMD128Vector)
+    : Prims.Pure t_SIMD128Vector Prims.l_True (fun _ -> Prims.l_True)
+
+val deserialize_1_ (a: u8) : Prims.Pure t_SIMD128Vector Prims.l_True (fun _ -> Prims.l_True)
+
+val from_i32_array (array: t_Array i32 (sz 8))
+    : Prims.Pure t_SIMD128Vector Prims.l_True (fun _ -> Prims.l_True)
+
+val inv_ntt_layer_1_step (v: t_SIMD128Vector) (zeta1 zeta2: i32)
+    : Prims.Pure t_SIMD128Vector Prims.l_True (fun _ -> Prims.l_True)
+
+val inv_ntt_layer_2_step (v: t_SIMD128Vector) (zeta: i32)
+    : Prims.Pure t_SIMD128Vector Prims.l_True (fun _ -> Prims.l_True)
+
+val montgomery_reduce (v: t_SIMD128Vector)
+    : Prims.Pure t_SIMD128Vector Prims.l_True (fun _ -> Prims.l_True)
+
+val multiply_by_constant (v: t_SIMD128Vector) (c: i32)
+    : Prims.Pure t_SIMD128Vector Prims.l_True (fun _ -> Prims.l_True)
+
+val ntt_layer_1_step (v: t_SIMD128Vector) (zeta1 zeta2: i32)
+    : Prims.Pure t_SIMD128Vector Prims.l_True (fun _ -> Prims.l_True)
+
+val ntt_layer_2_step (v: t_SIMD128Vector) (zeta: i32)
+    : Prims.Pure t_SIMD128Vector Prims.l_True (fun _ -> Prims.l_True)
+
+val ntt_multiply (lhs rhs: t_SIMD128Vector) (zeta0 zeta1: i32)
+    : Prims.Pure t_SIMD128Vector Prims.l_True (fun _ -> Prims.l_True)
+
+val serialize_1_ (v: t_SIMD128Vector) : Prims.Pure u8 Prims.l_True (fun _ -> Prims.l_True)
+
+val serialize_10_ (v: t_SIMD128Vector)
+    : Prims.Pure (t_Array u8 (sz 10)) Prims.l_True (fun _ -> Prims.l_True)
+
+val serialize_12_ (v: t_SIMD128Vector)
+    : Prims.Pure (t_Array u8 (sz 12)) Prims.l_True (fun _ -> Prims.l_True)
+
+val serialize_4_ (v: t_SIMD128Vector)
+    : Prims.Pure (t_Array u8 (sz 4)) Prims.l_True (fun _ -> Prims.l_True)
+
+val serialize_5_ (v: t_SIMD128Vector)
+    : Prims.Pure (t_Array u8 (sz 5)) Prims.l_True (fun _ -> Prims.l_True)
+
+val shift_left (v_SHIFT_BY: i32) (lhs: t_SIMD128Vector)
+    : Prims.Pure t_SIMD128Vector Prims.l_True (fun _ -> Prims.l_True)
+
+val shift_right (v_SHIFT_BY: i32) (v: t_SIMD128Vector)
+    : Prims.Pure t_SIMD128Vector Prims.l_True (fun _ -> Prims.l_True)
+
+val sub_vec (lhs rhs: t_SIMD128Vector)
+    : Prims.Pure t_SIMD128Vector Prims.l_True (fun _ -> Prims.l_True)
+
+val to_i32_array (v: t_SIMD128Vector)
+    : Prims.Pure (t_Array i32 (sz 8)) Prims.l_True (fun _ -> Prims.l_True)
+
+val deserialize_10_ (v: t_Slice u8)
+    : Prims.Pure t_SIMD128Vector Prims.l_True (fun _ -> Prims.l_True)
+
+val deserialize_11_ (v: t_Slice u8)
+    : Prims.Pure t_SIMD128Vector Prims.l_True (fun _ -> Prims.l_True)
+
+val deserialize_12_ (v: t_Slice u8)
+    : Prims.Pure t_SIMD128Vector Prims.l_True (fun _ -> Prims.l_True)
+
+val deserialize_4_ (v: t_Slice u8) : Prims.Pure t_SIMD128Vector Prims.l_True (fun _ -> Prims.l_True)
+
+val deserialize_5_ (v: t_Slice u8) : Prims.Pure t_SIMD128Vector Prims.l_True (fun _ -> Prims.l_True)
+
+val serialize_11_ (v: t_SIMD128Vector)
+    : Prims.Pure (t_Array u8 (sz 11)) Prims.l_True (fun _ -> Prims.l_True)
+
+[@@ FStar.Tactics.Typeclasses.tcinstance]
+let impl: Libcrux_ml_kem.Simd.Simd_trait.t_Operations t_SIMD128Vector =
+  {
+    f_ZERO_pre = (fun (_: Prims.unit) -> true);
+    f_ZERO_post = (fun (_: Prims.unit) (out: t_SIMD128Vector) -> true);
+    f_ZERO = (fun (_: Prims.unit) -> v_ZERO ());
+    f_to_i32_array_pre = (fun (v: t_SIMD128Vector) -> true);
+    f_to_i32_array_post = (fun (v: t_SIMD128Vector) (out: t_Array i32 (sz 8)) -> true);
+    f_to_i32_array = (fun (v: t_SIMD128Vector) -> to_i32_array v);
+    f_from_i32_array_pre = (fun (array: t_Array i32 (sz 8)) -> true);
+    f_from_i32_array_post = (fun (array: t_Array i32 (sz 8)) (out: t_SIMD128Vector) -> true);
+    f_from_i32_array = (fun (array: t_Array i32 (sz 8)) -> from_i32_array array);
+    f_add_constant_pre = (fun (v: t_SIMD128Vector) (c: i32) -> true);
+    f_add_constant_post = (fun (v: t_SIMD128Vector) (c: i32) (out: t_SIMD128Vector) -> true);
+    f_add_constant = (fun (v: t_SIMD128Vector) (c: i32) -> add_constant v c);
+    f_add_pre = (fun (lhs: t_SIMD128Vector) (rhs: t_SIMD128Vector) -> true);
+    f_add_post = (fun (lhs: t_SIMD128Vector) (rhs: t_SIMD128Vector) (out: t_SIMD128Vector) -> true);
+    f_add = (fun (lhs: t_SIMD128Vector) (rhs: t_SIMD128Vector) -> add_vec lhs rhs);
+    f_sub_pre = (fun (lhs: t_SIMD128Vector) (rhs: t_SIMD128Vector) -> true);
+    f_sub_post = (fun (lhs: t_SIMD128Vector) (rhs: t_SIMD128Vector) (out: t_SIMD128Vector) -> true);
+    f_sub = (fun (lhs: t_SIMD128Vector) (rhs: t_SIMD128Vector) -> sub_vec lhs rhs);
+    f_multiply_by_constant_pre = (fun (v: t_SIMD128Vector) (c: i32) -> true);
+    f_multiply_by_constant_post = (fun (v: t_SIMD128Vector) (c: i32) (out: t_SIMD128Vector) -> true);
+    f_multiply_by_constant = (fun (v: t_SIMD128Vector) (c: i32) -> multiply_by_constant v c);
+    f_bitwise_and_with_constant_pre = (fun (v: t_SIMD128Vector) (c: i32) -> true);
+    f_bitwise_and_with_constant_post
+    =
+    (fun (v: t_SIMD128Vector) (c: i32) (out: t_SIMD128Vector) -> true);
+    f_bitwise_and_with_constant
+    =
+    (fun (v: t_SIMD128Vector) (c: i32) -> bitwise_and_with_constant v c);
+    f_shift_right_pre = (fun (v_SHIFT_BY: i32) (v: t_SIMD128Vector) -> true);
+    f_shift_right_post = (fun (v_SHIFT_BY: i32) (v: t_SIMD128Vector) (out: t_SIMD128Vector) -> true);
+    f_shift_right = (fun (v_SHIFT_BY: i32) (v: t_SIMD128Vector) -> shift_right v_SHIFT_BY v);
+    f_shift_left_pre = (fun (v_SHIFT_BY: i32) (v: t_SIMD128Vector) -> true);
+    f_shift_left_post = (fun (v_SHIFT_BY: i32) (v: t_SIMD128Vector) (out: t_SIMD128Vector) -> true);
+    f_shift_left = (fun (v_SHIFT_BY: i32) (v: t_SIMD128Vector) -> shift_left v_SHIFT_BY v);
+    f_cond_subtract_3329_pre = (fun (v: t_SIMD128Vector) -> true);
+    f_cond_subtract_3329_post = (fun (v: t_SIMD128Vector) (out: t_SIMD128Vector) -> true);
+    f_cond_subtract_3329_ = (fun (v: t_SIMD128Vector) -> cond_subtract_3329_ v);
+    f_barrett_reduce_pre = (fun (v: t_SIMD128Vector) -> true);
+    f_barrett_reduce_post = (fun (v: t_SIMD128Vector) (out: t_SIMD128Vector) -> true);
+    f_barrett_reduce = (fun (v: t_SIMD128Vector) -> barrett_reduce v);
+    f_montgomery_reduce_pre = (fun (v: t_SIMD128Vector) -> true);
+    f_montgomery_reduce_post = (fun (v: t_SIMD128Vector) (out: t_SIMD128Vector) -> true);
+    f_montgomery_reduce = (fun (v: t_SIMD128Vector) -> montgomery_reduce v);
+    f_compress_1_pre = (fun (v: t_SIMD128Vector) -> true);
+    f_compress_1_post = (fun (v: t_SIMD128Vector) (out: t_SIMD128Vector) -> true);
+    f_compress_1_ = (fun (v: t_SIMD128Vector) -> compress_1_ v);
+    f_compress_pre = (fun (v_COEFFICIENT_BITS: i32) (v: t_SIMD128Vector) -> true);
+    f_compress_post
+    =
+    (fun (v_COEFFICIENT_BITS: i32) (v: t_SIMD128Vector) (out: t_SIMD128Vector) -> true);
+    f_compress
+    =
+    (fun (v_COEFFICIENT_BITS: i32) (v: t_SIMD128Vector) -> compress v_COEFFICIENT_BITS v);
+    f_ntt_layer_1_step_pre = (fun (a: t_SIMD128Vector) (zeta1: i32) (zeta2: i32) -> true);
+    f_ntt_layer_1_step_post
+    =
+    (fun (a: t_SIMD128Vector) (zeta1: i32) (zeta2: i32) (out: t_SIMD128Vector) -> true);
+    f_ntt_layer_1_step
+    =
+    (fun (a: t_SIMD128Vector) (zeta1: i32) (zeta2: i32) -> ntt_layer_1_step a zeta1 zeta2);
+    f_ntt_layer_2_step_pre = (fun (a: t_SIMD128Vector) (zeta: i32) -> true);
+    f_ntt_layer_2_step_post = (fun (a: t_SIMD128Vector) (zeta: i32) (out: t_SIMD128Vector) -> true);
+    f_ntt_layer_2_step = (fun (a: t_SIMD128Vector) (zeta: i32) -> ntt_layer_2_step a zeta);
+    f_inv_ntt_layer_1_step_pre = (fun (a: t_SIMD128Vector) (zeta1: i32) (zeta2: i32) -> true);
+    f_inv_ntt_layer_1_step_post
+    =
+    (fun (a: t_SIMD128Vector) (zeta1: i32) (zeta2: i32) (out: t_SIMD128Vector) -> true);
+    f_inv_ntt_layer_1_step
+    =
+    (fun (a: t_SIMD128Vector) (zeta1: i32) (zeta2: i32) -> inv_ntt_layer_1_step a zeta1 zeta2);
+    f_inv_ntt_layer_2_step_pre = (fun (a: t_SIMD128Vector) (zeta: i32) -> true);
+    f_inv_ntt_layer_2_step_post
+    =
+    (fun (a: t_SIMD128Vector) (zeta: i32) (out: t_SIMD128Vector) -> true);
+    f_inv_ntt_layer_2_step = (fun (a: t_SIMD128Vector) (zeta: i32) -> inv_ntt_layer_2_step a zeta);
+    f_ntt_multiply_pre
+    =
+    (fun (lhs: t_SIMD128Vector) (rhs: t_SIMD128Vector) (zeta0: i32) (zeta1: i32) -> true);
+    f_ntt_multiply_post
+    =
+    (fun
+        (lhs: t_SIMD128Vector)
+        (rhs: t_SIMD128Vector)
+        (zeta0: i32)
+        (zeta1: i32)
+        (out: t_SIMD128Vector)
+        ->
+        true);
+    f_ntt_multiply
+    =
+    (fun (lhs: t_SIMD128Vector) (rhs: t_SIMD128Vector) (zeta0: i32) (zeta1: i32) ->
+        ntt_multiply lhs rhs zeta0 zeta1);
+    f_serialize_1_pre = (fun (a: t_SIMD128Vector) -> true);
+    f_serialize_1_post = (fun (a: t_SIMD128Vector) (out: u8) -> true);
+    f_serialize_1_ = (fun (a: t_SIMD128Vector) -> serialize_1_ a);
+    f_deserialize_1_pre = (fun (a: u8) -> true);
+    f_deserialize_1_post = (fun (a: u8) (out: t_SIMD128Vector) -> true);
+    f_deserialize_1_ = (fun (a: u8) -> deserialize_1_ a);
+    f_serialize_4_pre = (fun (a: t_SIMD128Vector) -> true);
+    f_serialize_4_post = (fun (a: t_SIMD128Vector) (out: t_Array u8 (sz 4)) -> true);
+    f_serialize_4_ = (fun (a: t_SIMD128Vector) -> serialize_4_ a);
+    f_deserialize_4_pre = (fun (a: t_Slice u8) -> true);
+    f_deserialize_4_post = (fun (a: t_Slice u8) (out: t_SIMD128Vector) -> true);
+    f_deserialize_4_ = (fun (a: t_Slice u8) -> deserialize_4_ a);
+    f_serialize_5_pre = (fun (a: t_SIMD128Vector) -> true);
+    f_serialize_5_post = (fun (a: t_SIMD128Vector) (out: t_Array u8 (sz 5)) -> true);
+    f_serialize_5_ = (fun (a: t_SIMD128Vector) -> serialize_5_ a);
+    f_deserialize_5_pre = (fun (a: t_Slice u8) -> true);
+    f_deserialize_5_post = (fun (a: t_Slice u8) (out: t_SIMD128Vector) -> true);
+    f_deserialize_5_ = (fun (a: t_Slice u8) -> deserialize_5_ a);
+    f_serialize_10_pre = (fun (a: t_SIMD128Vector) -> true);
+    f_serialize_10_post = (fun (a: t_SIMD128Vector) (out: t_Array u8 (sz 10)) -> true);
+    f_serialize_10_ = (fun (a: t_SIMD128Vector) -> serialize_10_ a);
+    f_deserialize_10_pre = (fun (a: t_Slice u8) -> true);
+    f_deserialize_10_post = (fun (a: t_Slice u8) (out: t_SIMD128Vector) -> true);
+    f_deserialize_10_ = (fun (a: t_Slice u8) -> deserialize_10_ a);
+    f_serialize_11_pre = (fun (a: t_SIMD128Vector) -> true);
+    f_serialize_11_post = (fun (a: t_SIMD128Vector) (out: t_Array u8 (sz 11)) -> true);
+    f_serialize_11_ = (fun (a: t_SIMD128Vector) -> serialize_11_ a);
+    f_deserialize_11_pre = (fun (a: t_Slice u8) -> true);
+    f_deserialize_11_post = (fun (a: t_Slice u8) (out: t_SIMD128Vector) -> true);
+    f_deserialize_11_ = (fun (a: t_Slice u8) -> deserialize_11_ a);
+    f_serialize_12_pre = (fun (a: t_SIMD128Vector) -> true);
+    f_serialize_12_post = (fun (a: t_SIMD128Vector) (out: t_Array u8 (sz 12)) -> true);
+    f_serialize_12_ = (fun (a: t_SIMD128Vector) -> serialize_12_ a);
+    f_deserialize_12_pre = (fun (a: t_Slice u8) -> true);
+    f_deserialize_12_post = (fun (a: t_Slice u8) (out: t_SIMD128Vector) -> true);
+    f_deserialize_12_ = fun (a: t_Slice u8) -> deserialize_12_ a
+  }
